simplify proofs

coq/LC/Debruijn.v
@@ -162,6 +162,9 @@ Inductive parred : relation term :=
 Notation betared := [* betared1].
 Infix "->b" := betared (at level 70, no associativity).
 
+Hint Resolve betared1beta betared1appl betared1appr betared1abs
+    parredvar parredapp parredabs parredbeta.
+
 Function reduce_all_redex t : term :=
   match t with
     | var _ => t
@@ -173,32 +176,32 @@ Function reduce_all_redex t : term :=
 
 Lemma parred_refl : forall t, parred t t.
 Proof.
-  by elim; constructor.
+  elim; auto.
 Qed.
 
 Lemma betaredappl : forall t1 t1' t2, t1 ->b t1' -> app t1 t2 ->b app t1' t2.
 Proof.
   move => t1 t1' t2; elim => // {t1 t1'} t1 t1' t1'' ? ? ?.
-  by apply rt1n_trans with (app t1' t2) => //; constructor.
+  apply rt1n_trans with (app t1' t2) => //; auto.
 Qed.
 
 Lemma betaredappr : forall t1 t2 t2', t2 ->b t2' -> app t1 t2 ->b app t1 t2'.
 Proof.
   move => t1 t2 t2'; elim => // {t2 t2'} t2 t2' t2'' ? ? ?.
-  by apply rt1n_trans with (app t1 t2') => //; constructor.
+  apply rt1n_trans with (app t1 t2') => //; auto.
 Qed.
 
 Lemma betaredabs : forall t t', t ->b t' -> abs t ->b abs t'.
 Proof.
   move => t t'; elim => // {t t'} t t' t'' ? ? ?.
-  by apply rt1n_trans with (abs t') => //; constructor.
+  apply rt1n_trans with (abs t') => //; auto.
 Qed.
 
 Hint Resolve parred_refl betaredappl betaredappr betaredabs.
 
 Lemma betared1_in_parred : inclusion betared1 parred.
 Proof.
-  by apply betared1_ind; constructor.
+  apply betared1_ind; auto.
 Qed.
 
 Lemma parred_in_betared : inclusion parred betared.
@@ -209,7 +212,7 @@ Proof.
   - move => t1 t1' t2 t2' ? ? ? ?.
     apply rtc_trans' with (app (abs t1') t2); auto.
     apply rtc_trans' with (app (abs t1') t2'); auto.
-    apply rtc_step; constructor.
+    by apply rtc_step.
 Qed.
 
 Lemma subst_betared1 :
@@ -217,20 +220,16 @@ Lemma subst_betared1 :
   t2 ->1b t2' -> substitute n t1 t2 ->1b substitute n t1 t2'.
 Proof.
   move => n t1 t2 t2' H; move: t2 t2' H n.
-  refine (betared1_ind _ _ _ _ _); try by constructor.
-  move => t2 t2' n.
-  rewrite (subst_subst_distr n 0).
-  constructor.
+  refine (betared1_ind _ _ _ _ _) => /=; auto => t2 t2' n.
+  by rewrite (subst_subst_distr n 0).
 Qed.
 
 Lemma shift_parred :
   forall t t' d c, t ->bp t' -> shift d c t ->bp shift d c t'.
 Proof.
   move => t t' d c H; move: t t' H d c.
-  refine (parred_ind _ _ _ _ _) => //; try by constructor.
-  move => t1 t1' t2 t2' ? ? ? ? d c /=.
-  rewrite (subst_shift_distr 0).
-  by constructor.
+  refine (parred_ind _ _ _ _ _) => //=; auto => t1 t1' t2 t2' ? ? ? ? d c.
+  rewrite (subst_shift_distr 0); auto.
 Qed.
 
 Lemma subst_parred :
@@ -238,10 +237,10 @@ Lemma subst_parred :
   t1 ->bp t1' -> t2 ->bp t2' -> substitute n t1 t2 ->bp substitute n t1' t2'.
 Proof.
   move => n t1 t1' t2 t2' H H0; move: t2 t2' H0 n.
-  refine (parred_ind _ _ _ _ _) => /=; try constructor; auto.
+  refine (parred_ind _ _ _ _ _) => /=; auto.
   - by move => m n; elimif; apply shift_parred.
   - move => t2l t2l' ? ? t2r t2r' ? ? n.
-    by rewrite (subst_subst_distr n 0); constructor.
+    rewrite (subst_subst_distr n 0); auto.
 Qed.
 
 Lemma parred_all_lemma : forall t t', t ->bp t' -> t' ->bp reduce_all_redex t.
@@ -249,10 +248,10 @@ Proof with auto.
   move => t; elim/reduce_all_redex_ind: {t}_.
   - by move => t n ? t' H; inversion H; subst.
   - move => _ t1 t2 _ ? ? t' H; inversion H; subst.
-    - inversion H2; subst; constructor...
+    - inversion H2; subst...
     - apply subst_parred...
-  - move => _ t1 t2 _ ? ? ? t' H; inversion H; subst => //; constructor...
-  - move => _ t1 _ ? t2 H; inversion H; subst; constructor...
+  - move => _ t1 t2 _ ? ? ? t' H; inversion H; subst => //...
+  - move => _ t1 _ ? t2 H; inversion H; subst...
 Qed.
 
 Lemma parred_confluent : confluent parred.
@@ -279,6 +278,8 @@ Inductive typing : context typ -> term -> typ -> Prop :=
   | typabs : forall ctx t ty1 ty2,
     typing (Some ty1 :: ctx) t ty2 -> typing ctx (abs t) (tyfun ty1 ty2).
 
+Hint Resolve typvar typapp typabs.
+
 Lemma typvar_seqindex :
   forall ctx n ty, typing ctx (var n) ty <-> ctxindex ctx n ty.
 Proof.
@@ -293,10 +294,8 @@ Lemma ctxleq_preserves_typing :
 Proof.
   move => ctx1 ctx2 t ty H H0; move: ctx1 t ty H0 ctx2 H.
   refine (typing_ind _ _ _ _).
-  - move => ctx2 n ty H ctx1 H0.
-    constructor; auto.
-  - move => ctx2 tl tr tyl tyr H H0 H1 H2 ctx1 H3.
-    apply typapp with tyl; auto.
+  - auto.
+  - eauto.
   - move => ctx2 t tyl tyr H H0 ctx1 H1.
     by constructor; apply H0; case.
 Qed.
@@ -309,8 +308,7 @@ Proof.
   refine (typing_ind _ _ _ _).
   - move => /= ctx1 n ty H c ctx2.
     rewrite typvar_seqindex H ctxnth_ctxinsert; elimif_omega.
-  - move => /= ctx t1 t2 ty1 ty2 H H0 H1 H2 c ctx2.
-    apply typapp with ty1; auto.
+  - simpl; eauto.
   - move => /= ctx1 t ty1 ty2 H H0 c ctx2.
     constructor; apply (H0 c.+1).
 Qed.
@@ -320,7 +318,7 @@ Lemma subject_substitute_seq :
   Forall (fun p => typing (drop n ctx) p.1 p.2) ctx' ->
   typing (ctxinsert [seq Some p.2 | p <- ctx'] ctx n) t ty ->
   typing ctx (substitute_seq n [seq p.1 | p <- ctx'] t) ty.
-Proof.
+Proof with auto.
   elim.
   - move => /= m ty n ctx ctx'.
     rewrite /substitute_seqv typvar_seqindex ctxnth_ctxinsert !size_map.
@@ -341,11 +339,9 @@ Proof.
       - rewrite typvar_seqindex H3; f_equal; ssromega.
       - rewrite size_map; ssromega.
   - move => tl IHtl tr IHtr ty n ctx ctx' H H0.
-    inversion H0; subst => /= {H0}.
-    apply typapp with ty1; auto.
+    inversion H0; subst => /= {H0}; apply typapp with ty1...
   - move => /= t IH ty n ctx ctx' H H0.
-    inversion H0; subst => {H0}.
-    constructor; auto.
+    inversion H0; subst => {H0}...
 Qed.
 
 Lemma subject_reduction :
@@ -360,13 +356,11 @@ Proof.
     - by rewrite /= drop0.
     - by rewrite /ctxinsert sub0n take0 drop0 /=.
   - move => t1 t1' t2 H IH ctx ty H0.
-    inversion H0; subst.
-    by apply typapp with ty1; auto.
+    inversion H0; subst; eauto.
   - move => t1 t2 t2' H IH ctx ty H0.
-    inversion H0; subst.
-    by apply typapp with ty1; auto.
+    inversion H0; subst; eauto.
   - move => t1 t2 H IH ctx ty H0.
-    inversion H0; subst; constructor; auto.
+    inversion H0; subst; auto.
 Qed.
 
 Notation SNorm t := (Acc (fun x y => betared1 y x) t).
@@ -378,15 +372,13 @@ Proof.
   by apply IH, H; constructor.
 Qed.
 
-Fixpoint reducible' (ctx : context typ) (t : term) (ty : typ) : Prop :=
+Fixpoint reducible (ctx : context typ) (t : term) (ty : typ) : Prop :=
   match ty with
     | tyvar n => SNorm t
     | tyfun ty1 ty2 => forall t1 ctx',
-        ctxleq ctx ctx' -> typing ctx' t1 ty1 /\ reducible' ctx' t1 ty1 ->
-        reducible' ctx' (app t t1) ty2
+        ctxleq ctx ctx' -> typing ctx' t1 ty1 -> reducible ctx' t1 ty1 ->
+        reducible ctx' (app t t1) ty2
   end.
-
-Notation reducible ctx t ty := (typing ctx t ty /\ reducible' ctx t ty).
 
 Definition neutral t := (if t is abs _ then False else True).
 
@@ -394,66 +386,56 @@ Lemma ctxleq_preserves_reducibility :
   forall ctx ctx' t ty,
   ctxleq ctx ctx' -> reducible ctx t ty -> reducible ctx' t ty.
 Proof.
-  move => ctx ctx' tl ty H [H0 H1]; split.
-  - by apply ctxleq_preserves_typing with ctx.
-  - case: ty H H0 H1 => //= tyl tyr H H0 H1 tr ctx'' H2.
-    apply H1; auto.
+  move => ctx ctx' t [] //=; auto.
 Qed.
-
-Lemma CR2' :
-  forall ctx t t' ty, t ->1b t' -> reducible' ctx t ty -> reducible' ctx t' ty.
-Proof.
-  move => ctx t t' ty; elim: ty ctx t t'.
-  - by move => /= n ctx t1 t2 H []; apply.
-  - move => /= tyl IHtyl tyr IHtyr ctx t1 t2 H H0 t3 ctx' H1 H2.
-    by apply IHtyr with (app t1 t3); auto; constructor.
-Qed.
-
-Arguments CR2' [ctx t t' ty] _ _.
 
 Lemma CR2 :
   forall ctx t t' ty, t ->1b t' -> reducible ctx t ty -> reducible ctx t' ty.
 Proof.
-  move => ctx t t' ty H [H0 H1].
-  exact (conj (subject_reduction H H0) (CR2' H H1)).
+  move => ctx t t' ty; elim: ty ctx t t'.
+  - by move => /= _ _ t t' H []; apply.
+  - move => /= tyl IHtyl tyr IHtyr ctx t1 t2 H H0 t3 ctx' H1 H2 H3.
+    by apply IHtyr with (app t1 t3); auto; constructor.
 Qed.
+
+Arguments CR2 [ctx t t' ty] _ _.
 
 Lemma CR1_and_CR3 :
   forall ty,
-  (forall ctx t, reducible ctx t ty -> SNorm t) /\
+  (forall ctx t, typing ctx t ty -> reducible ctx t ty -> SNorm t) /\
   (forall ctx t, typing ctx t ty -> neutral t ->
-   (forall t', t ->1b t' -> reducible' ctx t' ty) -> reducible' ctx t ty).
+   (forall t', t ->1b t' -> reducible ctx t' ty) -> reducible ctx t ty).
 Proof.
   elim.
   - move => n; split => /= ctx t.
     - firstorder.
     - move => H H0 H1; constructor; firstorder.
   - move => tyl [IHtyl1 IHtyl2] tyr [IHtyr1 IHtyr2] /=.
-    split => [ctx t [H H0] | ctx t H H0 H1 tr ctx' H2 H3].
+    split => [ctx t H H0 | ctx tl H H0 H1 tr ctx' H2 H3 H4].
     - have H1: typing (ctx ++ [:: Some tyl]) (size ctx) tyl
         by rewrite typvar_seqindex nth_cat ltnn subnn.
       have H2: typing (ctx ++ [:: Some tyl]) (app t (size ctx)) tyr
         by apply typapp with tyl => //; move: H;
         apply ctxleq_preserves_typing, ctxleq_appr.
-      apply snorm_appl with (size ctx),
-        IHtyr1 with (ctx ++ [:: Some tyl]), (conj H2), IHtyr2 => // t' H3.
-      apply (CR2' H3), H0.
+      apply snorm_appl with (size ctx), (IHtyr1 _ _ H2), IHtyr2 => // t' H3.
+      apply (CR2 H3), H0 => //.
       - apply ctxleq_appr.
-      - apply (conj H1), IHtyl2 => // x H4; inversion H4.
-    - have H4: SNorm tr by apply IHtyl1 with ctx'.
-      move: tr H4 H2 H3; refine (Acc_ind _ _) => tr _ IH H2 [H3 H4].
-      have H5: typing ctx' (app t tr) tyr.
+      - apply IHtyl2 => // x H4; inversion H4.
+    - have H5: SNorm tr by apply IHtyl1 with ctx' => //.
+      move: tr H5 H2 H3 H4; refine (Acc_ind _ _) => tr _ IH H2 H3 H4.
+      have H5: typing ctx' (app tl tr) tyr.
         apply typapp with tyl.
         - by apply ctxleq_preserves_typing with ctx.
         - tauto.
-      apply IHtyr2 => // tr' H6.
+      apply IHtyr2 => // t' H6.
       move: H0; inversion H6; subst => // _.
       - by apply H1.
       - apply IH => //.
-        by apply (conj (subject_reduction H9 H3)), CR2' with tr.
+        - by move: H3; apply subject_reduction.
+        - by move: H4; apply CR2.
 Qed.
 
-Lemma CR1 : forall ctx t ty, reducible ctx t ty -> SNorm t.
+Lemma CR1 : forall ctx t ty, typing ctx t ty -> reducible ctx t ty -> SNorm t.
 Proof.
   move => ctx t ty; case: (CR1_and_CR3 ty); firstorder.
 Qed.
@@ -463,7 +445,7 @@ Lemma CR3 :
   (forall t', t ->1b t' -> reducible ctx t' ty) -> reducible ctx t ty.
 Proof.
   move => ctx t ty; case: (CR1_and_CR3 ty) => _ H H0 H1 H2.
-  apply (conj H0), H => //; apply H2.
+  apply H => //; apply H2.
 Qed.
 
 Lemma snorm_subst : forall t1 t2, SNorm (substitute 0 t2 t1) -> SNorm t1.
@@ -478,32 +460,38 @@ Qed.
 Lemma abstraction_lemma :
   forall ctx t1 tyl tyr,
   typing ctx (abs t1) (tyfun tyl tyr) ->
-  (forall t2 ctx', ctxleq ctx ctx' ->
+  (forall t2 ctx', ctxleq ctx ctx' -> typing ctx' t2 tyl ->
    reducible ctx' t2 tyl -> reducible ctx' (substitute 0 t2 t1) tyr) ->
   reducible ctx (abs t1) (tyfun tyl tyr).
 Proof.
-  move => ctx t1 tyl tyr H H0; split => //= t2 ctx' H1 H2.
-  suff: (reducible ctx' (app (abs t1) t2) tyr) by tauto.
-  move: (snorm_subst t1 t2 (CR1 (H0 t2 ctx' H1 H2))) (CR1 H2) => H3 H4.
-  move: t1 H3 t2 H4 H H0 H1 H2.
-  refine (Acc_ind _ _) => t1 H H0; refine (Acc_ind _ _) => t2 H1 H2 H3 H4 H5 H6.
+  move => /= ctx t1 tyl tyr H H0 t2 ctx' H1 H2 H3.
+  have H4: (typing ctx' (substitute 0 t2 t1) tyr).
+    apply subject_reduction with (app (abs t1) t2); auto.
+    apply typapp with tyl => //.
+    by move: H; apply ctxleq_preserves_typing.
+  move: (snorm_subst t1 t2 (CR1 H4 (H0 t2 ctx' H1 H2 H3))) (CR1 H2 H3) => H5 H6.
+  move: t1 H5 t2 H6 H H0 H1 H2 H3 {H4}.
+  refine (Acc_ind _ _) => t1 H H0.
+  refine (Acc_ind _ _) => t2 H1 H2 H3 H4 H5 H6 H7.
   apply CR3 => //.
-  - apply typapp with tyl.
-    - by apply ctxleq_preserves_typing with ctx.
-    - tauto.
-  - move => t3 H7.
-    inversion H7; subst => {H7}; auto.
-    - inversion H11; subst => {H11}.
+  - apply typapp with tyl => //.
+    by apply ctxleq_preserves_typing with ctx.
+  - move => t3 H8.
+    inversion H8; subst => {H8}; auto.
+    - inversion H12; subst => {H12}.
       apply H0 => //.
-      - by apply subject_reduction with (abs t1) => //; constructor.
-      - by move => t'' ctx'' H7 H9; apply (CR2 (subst_betared1 0 t'' H8)), H4.
-    - by apply H2 => //; apply CR2 with t2.
+      - by apply subject_reduction with (abs t1); auto.
+      - by move => t'' ctx'' H8 H10 H11;
+          apply (CR2 (subst_betared1 0 t'' H9)), H4.
+    - apply H2 => //.
+      - by apply subject_reduction with t2.
+      - by apply CR2 with t2.
 Qed.
 
 Lemma reduce_lemma :
   forall ctx (ctx' : seq (term * typ)) t ty,
   typing ([seq Some p.2 | p <- ctx'] ++ ctx) t ty ->
-  Forall (fun p => reducible ctx p.1 p.2) ctx' ->
+  Forall (fun p => typing ctx p.1 p.2 /\ reducible ctx p.1 p.2) ctx' ->
   reducible ctx (substitute_seq 0 [seq p.1 | p <- ctx'] t) ty.
 Proof.
   move => ctx ctx' t ty; elim: t ty ctx ctx'.
@@ -511,39 +499,37 @@ Proof.
     rewrite /substitute_seqv typvar_seqindex subn0 size_map shiftzero.
     elim: ctx' n => [| c' ctx' IH []] /=.
     - move => n H _; rewrite nth_nil subn0.
-      apply CR3 => //.
-      - by constructor.
-      - move => t' H0; inversion H0.
-    - by case => H [H0 H1]; rewrite H.
-    - by move => n H [H0 H1]; apply IH.
+      apply CR3 => //; auto => t' H0; inversion H0.
+    - by move => [->] [[_ H] _].
+    - by move => n H [_ H0]; apply IH.
   - move => tl IHtl tr IHtr ty ctx ctx' H H0.
     inversion H; subst => {H}.
-    case: (IHtl (tyfun ty1 ty) ctx ctx') => //= H1 H2; split; auto.
-    apply typapp with ty1 => //.
+    move: (IHtl (tyfun ty1 ty) ctx ctx') => /=; apply; auto.
     apply subject_substitute_seq.
-    - by rewrite drop0; move: H0; apply Forall_impl => p [].
+    - rewrite drop0; move: H0; apply Forall_impl; tauto.
     - by rewrite /ctxinsert sub0n take0 drop0 /=.
   - move => t IHt ty ctx ctx' H H0.
     inversion H; subst => {H} /=.
     apply abstraction_lemma.
     - constructor.
       apply subject_substitute_seq.
-      - by rewrite /= drop0; move: H0; apply Forall_impl => p [].
+      - rewrite /= drop0; move: H0; apply Forall_impl; tauto.
       - by rewrite /ctxinsert /= take0 drop0 /=.
-    - move => t2 ctx2 H H1.
+    - move => t2 ctx2 H H1 H2.
       rewrite substitute_seq_cons_eq.
       apply (IHt ty2 ctx2 ((t2, ty1) :: ctx')) => /=.
       - move: H3; apply ctxleq_preserves_typing.
         move: H; apply (ctxleq_appl (Some ty1 :: _)).
       - split => //.
-        move: H0; apply Forall_impl => p.
-        by apply ctxleq_preserves_reducibility.
+        move: H0; apply Forall_impl => p [H4 H5]; split.
+        - by move: H4; apply ctxleq_preserves_typing.
+        - by move: H5; apply ctxleq_preserves_reducibility.
 Qed.
 
 Theorem typed_term_is_snorm : forall ctx t ty, typing ctx t ty -> SNorm t.
 Proof.
   move => ctx t ty H.
-  apply (@CR1 ctx t ty).
+  apply (@CR1 ctx t ty) => //.
   move: (@reduce_lemma ctx [::] t ty H) => /=.
   by rewrite substitute_seq_nil_eq; apply.
 Qed.
